verbs/library/music/scores/unknown.ly
@@ -1,0 +1,42 @@
+<!DOCTYPE HTML PUBLIC "-//W3C//DTD HTML 3.2 Final//EN">
+<html>
+ <head>
+  <title>Index of /ftp/MozartWA/KV620/magicflute-07-duet/magicflute-07-duet-lys</title>
+ </head>
+ <body>
+<h1>Index of /ftp/MozartWA/KV620/magicflute-07-duet/magicflute-07-duet-lys</h1>
+  <table>
+   <tr><th valign="top"><img src="/icons/blank.gif" alt="[ICO]"></th><th><a href="?C=N;O=D">Name</a></th><th><a href="?C=M;O=A">Last modified</a></th><th><a href="?C=S;O=A">Size</a></th><th><a href="?C=D;O=A">Description</a></th></tr>
+   <tr><th colspan="5"><hr></th></tr>
+<tr><td valign="top"><img src="/icons/back.gif" alt="[PARENTDIR]"></td><td><a href="/ftp/MozartWA/KV620/magicflute-07-duet/">Parent Directory</a></td><td>&nbsp;</td><td align="right">  - </td><td>&nbsp;</td></tr>
+<tr><td valign="top"><img src="/icons/text.gif" alt="[TXT]"></td><td><a href="MF7-Duett.ly">MF7-Duett.ly</a></td><td align="right">2013-03-26 05:59  </td><td align="right"> 12K</td><td>&nbsp;</td></tr>
+<tr><td valign="top"><img src="/icons/text.gif" alt="[TXT]"></td><td><a href="MF7-DuettScore.ly">MF7-DuettScore.ly</a></td><td align="right">2013-03-26 06:00  </td><td align="right"> 85 </td><td>&nbsp;</td></tr>
+<tr><td valign="top"><img src="/icons/text.gif" alt="[TXT]"></td><td><a href="clarinetti.ly">clarinetti.ly</a></td><td align="right">2013-03-26 06:00  </td><td align="right">112 </td><td>&nbsp;</td></tr>
+<tr><td valign="top"><img src="/icons/unknown.gif" alt="[   ]"></td><td><a href="clarinettib.ily">clarinettib.ily</a></td><td align="right">2013-03-26 06:00  </td><td align="right">225 </td><td>&nbsp;</td></tr>
+<tr><td valign="top"><img src="/icons/unknown.gif" alt="[   ]"></td><td><a href="contrabasso.ily">contrabasso.ily</a></td><td align="right">2013-03-26 06:00  </td><td align="right">173 </td><td>&nbsp;</td></tr>
+<tr><td valign="top"><img src="/icons/text.gif" alt="[TXT]"></td><td><a href="contrabasso.ly">contrabasso.ly</a></td><td align="right">2013-03-26 06:00  </td><td align="right">112 </td><td>&nbsp;</td></tr>
+<tr><td valign="top"><img src="/icons/text.gif" alt="[TXT]"></td><td><a href="corni.ly">corni.ly</a></td><td align="right">2013-03-26 06:00  </td><td align="right">107 </td><td>&nbsp;</td></tr>
+<tr><td valign="top"><img src="/icons/unknown.gif" alt="[   ]"></td><td><a href="cornie.ily">cornie.ily</a></td><td align="right">2013-03-26 06:00  </td><td align="right">170 </td><td>&nbsp;</td></tr>
+<tr><td valign="top"><img src="/icons/unknown.gif" alt="[   ]"></td><td><a href="fagotti.ily">fagotti.ily</a></td><td align="right">2013-03-26 06:00  </td><td align="right">162 </td><td>&nbsp;</td></tr>
+<tr><td valign="top"><img src="/icons/text.gif" alt="[TXT]"></td><td><a href="fagotti.ly">fagotti.ly</a></td><td align="right">2013-03-26 06:00  </td><td align="right">108 </td><td>&nbsp;</td></tr>
+<tr><td valign="top"><img src="/icons/text.gif" alt="[TXT]"></td><td><a href="header.ly">header.ly</a></td><td align="right">2013-03-26 06:00  </td><td align="right">2.9K</td><td>&nbsp;</td></tr>
+<tr><td valign="top"><img src="/icons/text.gif" alt="[TXT]"></td><td><a href="midi.ly">midi.ly</a></td><td align="right">2013-03-26 06:00  </td><td align="right">107 </td><td>&nbsp;</td></tr>
+<tr><td valign="top"><img src="/icons/unknown.gif" alt="[   ]"></td><td><a href="pamina.ily">pamina.ily</a></td><td align="right">2013-03-26 06:00  </td><td align="right">147 </td><td>&nbsp;</td></tr>
+<tr><td valign="top"><img src="/icons/text.gif" alt="[TXT]"></td><td><a href="pamina.ly">pamina.ly</a></td><td align="right">2013-03-26 06:00  </td><td align="right">107 </td><td>&nbsp;</td></tr>
+<tr><td valign="top"><img src="/icons/unknown.gif" alt="[   ]"></td><td><a href="papageno.ily">papageno.ily</a></td><td align="right">2013-03-26 06:00  </td><td align="right">172 </td><td>&nbsp;</td></tr>
+<tr><td valign="top"><img src="/icons/text.gif" alt="[TXT]"></td><td><a href="papageno.ly">papageno.ly</a></td><td align="right">2013-03-26 06:00  </td><td align="right">109 </td><td>&nbsp;</td></tr>
+<tr><td valign="top"><img src="/icons/text.gif" alt="[TXT]"></td><td><a href="piece.ly">piece.ly</a></td><td align="right">2013-03-26 06:00  </td><td align="right">265 </td><td>&nbsp;</td></tr>
+<tr><td valign="top"><img src="/icons/unknown.gif" alt="[   ]"></td><td><a href="score.ily">score.ily</a></td><td align="right">2013-03-26 06:00  </td><td align="right">1.1K</td><td>&nbsp;</td></tr>
+<tr><td valign="top"><img src="/icons/unknown.gif" alt="[   ]"></td><td><a href="staff.ily">staff.ily</a></td><td align="right">2013-03-26 06:00  </td><td align="right">204 </td><td>&nbsp;</td></tr>
+<tr><td valign="top"><img src="/icons/unknown.gif" alt="[   ]"></td><td><a href="viola.ily">viola.ily</a></td><td align="right">2013-03-26 06:00  </td><td align="right">128 </td><td>&nbsp;</td></tr>
+<tr><td valign="top"><img src="/icons/text.gif" alt="[TXT]"></td><td><a href="viola.ly">viola.ly</a></td><td align="right">2013-03-26 06:00  </td><td align="right">106 </td><td>&nbsp;</td></tr>
+<tr><td valign="top"><img src="/icons/unknown.gif" alt="[   ]"></td><td><a href="violinoI.ily">violinoI.ily</a></td><td align="right">2013-03-26 06:00  </td><td align="right">129 </td><td>&nbsp;</td></tr>
+<tr><td valign="top"><img src="/icons/text.gif" alt="[TXT]"></td><td><a href="violinoI.ly">violinoI.ly</a></td><td align="right">2013-03-26 06:00  </td><td align="right">109 </td><td>&nbsp;</td></tr>
+<tr><td valign="top"><img src="/icons/unknown.gif" alt="[   ]"></td><td><a href="violinoII.ily">violinoII.ily</a></td><td align="right">2013-03-26 06:01  </td><td align="right">133 </td><td>&nbsp;</td></tr>
+<tr><td valign="top"><img src="/icons/text.gif" alt="[TXT]"></td><td><a href="violinoII.ly">violinoII.ly</a></td><td align="right">2013-03-26 06:01  </td><td align="right">110 </td><td>&nbsp;</td></tr>
+<tr><td valign="top"><img src="/icons/unknown.gif" alt="[   ]"></td><td><a href="violoncello.ily">violoncello.ily</a></td><td align="right">2013-03-26 06:01  </td><td align="right">151 </td><td>&nbsp;</td></tr>
+<tr><td valign="top"><img src="/icons/text.gif" alt="[TXT]"></td><td><a href="violoncello.ly">violoncello.ly</a></td><td align="right">2013-03-26 06:01  </td><td align="right">112 </td><td>&nbsp;</td></tr>
+   <tr><th colspan="5"><hr></th></tr>
+</table>
+<address>Apache/2.4.58 (Ubuntu) Server at www.mutopiaproject.org Port 443</address>
+</body></html>
